Defining makeC

TypeSoundness.v
@@ -106,6 +106,21 @@ Infix "×" := Tprod (at level 40).
 Infix "+" := Tsum.
 Notation "e ↓ τ" := (IsValue e /\ |~ [] e τ) (at level 51).
 
+Definition sound_wrt_bounded :=
+  forall f τ₁ c s τ₂, 
+    f ↓ Tarrow τ₁ c s τ₂ -> 
+    exists (C : nat) (ξ₀ : csize), 
+      (* ξ₀ is the threshold of input size in asymptotics *)
+      forall v,
+        v ↓ τ₁ ->
+        let ξ := |v| in
+        ξ₀ <= ξ ->
+        forall v' n, 
+          (* n is the actual running time *)
+          ⇓ (Eapp f v) n v' ->
+          (* n is bounded by c(ξ) w.r.t. constant factor C *)
+          ⌊ ñ | n <= C * ñ ⌋ (subst ξ c).
+
 (* A Parametric Higher-Order Abstract Syntax (PHOAS) encoding for a second-order modal logic (LSLR) *)
 
 Section rel.
@@ -114,7 +129,7 @@ Section rel.
   
   Inductive rel : nat -> Type :=
   | Rvar n : var n -> rel n
-  | Rlift : Prop -> rel 0
+  | Rinj : Prop -> rel 0
   | Rtrue : rel 0
   | Rfalse : rel 0
   | Rand (_ _ : rel 0) : rel 0
@@ -134,6 +149,8 @@ Section rel.
 
 End rel.
 
+Module ClosedPHOAS.
+
 Notation "⊤" := (Rtrue _).
 Notation "⊥" := (Rtrue _).
 (* Notation "\ e , p" := (Rabs (fun e => p)) (at level 200, format "\ e , p"). *)
@@ -148,7 +165,7 @@ Definition RexistsR' var n P := (@RexistsR var n (fun x => P (Rvar _ _ x))).
 Notation "∃2 x .. y , p" := (RexistsR' (fun x => .. (RexistsR' (fun y => p)) ..)) (at level 200, x binder, y binder, right associativity).
 Definition Rrecur' var n P := (@Rrecur var n (fun x => P (Rvar _ _ x))).
 Notation "@ x .. y , p" := (Rrecur' (fun x => .. (Rrecur' (fun y => p)) ..)) (at level 200, x binder, y binder, right associativity).
-Notation "⌈ P ⌉" := (Rlift _ P).
+Notation "⌈ P ⌉" := (Rinj _ P).
 Notation "e ∈ P" := (Rapp P e) (at level 70).
 Infix "/\" := Rand.
 Infix "\/" := Ror.
@@ -256,21 +273,42 @@ Section LR.
   Definition E := E' V.
 
 End LR.
-(*
+
+End ClosedPHOAS.
+
+Module OpenPHOAS.
+
 Section relOpen.
 
   Variable var : nat -> Type.
   
-  Fixpoint relOpen R n :=
-    match R with
-      | nil => rel var n 
-      | nv :: R' => var nv -> relOpen R' n
+  Inductive termType :=
+    | TTrel (arity : nat)
+    | TTexpr
+    | TTother (T : Type)
+  .
+
+  Coercion TTrel : nat >-> termType.
+
+  Definition interp t :=
+    match t with
+      | TTrel n => rel var n
+      | TTexpr => expr
+      | TTother T => T
     end.
 
-  Program Fixpoint liftToOpen R n1 n2 (f : rel var n1 -> rel var n2) (a : relOpen R n1) : relOpen R n2 :=
-    match R with
+  Definition Ctx := list termType.
+
+  Fixpoint relOpen C range :=
+    match C with
+      | nil => interp range
+      | domain :: C' => interp domain -> relOpen C' range
+    end.
+
+  Program Fixpoint liftToOpen C n1 n2 (f : rel var n1 -> rel var n2) (a : relOpen C n1) : relOpen C n2 :=
+    match C with
       | nil => _
-      | nv :: R' => _ (@liftToOpen R' n1 n2)
+      | nv :: C' => _ (@liftToOpen C' n1 n2)
     end.
   Next Obligation.
     exact (f a).
@@ -281,10 +319,10 @@ Section relOpen.
 
   Require Import Program.
 
-  Program Fixpoint liftToOpen2 R n1 n2 T (f : (T -> rel var n1) -> rel var n2) (a : T -> relOpen R n1) : relOpen R n2 :=
-    match R with
+  Program Fixpoint liftToOpen2 C n1 n2 T (f : (T -> rel var n1) -> rel var n2) (a : T -> relOpen C n1) : relOpen C n2 :=
+    match C with
       | nil => _
-      | nv :: R' => _ (@liftToOpen2 R' n1 n2)
+      | nv :: C' => _ (@liftToOpen2 C' n1 n2)
     end.
   Next Obligation.
     exact (f a).
@@ -293,22 +331,22 @@ Section relOpen.
     exact (x _ f (flip a X)).
   Defined.
 
-  Program Fixpoint liftToOpen3 R n T (f : T -> rel var n) (a : T) : relOpen R n :=
-    match R with
+  Program Fixpoint liftToOpen3 C n T (f : T -> rel var n) (a : T) : relOpen C n :=
+    match C with
       | nil => _
-      | nv :: R' => _ (@liftToOpen3 R' n)
+      | nv :: C' => _ (@liftToOpen3 C' n)
     end.
 
-  Program Fixpoint liftToOpen4 R n (f : rel var n) : relOpen R n :=
-    match R with
+  Program Fixpoint liftToOpen4 C n (f : rel var n) : relOpen C n :=
+    match C with
       | nil => _
-      | nv :: R' => _ (@liftToOpen4 R' n)
+      | nv :: C' => _ (@liftToOpen4 C' n)
     end.
 
-  Program Fixpoint liftToOpen5 R n1 n2 n3 (f : rel var n1 -> rel var n2 -> rel var n3) (a : relOpen R n1) (b : relOpen R n2) : relOpen R n3 :=
-    match R with
+  Program Fixpoint liftToOpen5 C n1 n2 n3 (f : rel var n1 -> rel var n2 -> rel var n3) (a : relOpen C n1) (b : relOpen C n2) : relOpen C n3 :=
+    match C with
       | nil => _
-      | nv :: R' => _ (@liftToOpen5 R' n1 n2 n3)
+      | nv :: C' => _ (@liftToOpen5 C' n1 n2 n3)
     end.
   Next Obligation.
     exact (f a b).
@@ -317,10 +355,10 @@ Section relOpen.
     exact (x f (a X) (b X)).
   Defined.
 
-  Program Fixpoint liftToOpen6 R n1 T n2 (f : rel var n1 -> T -> rel var n2) (a : relOpen R n1) (b : T) : relOpen R n2 :=
-    match R with
+  Program Fixpoint liftToOpen6 C n1 T n2 (f : rel var n1 -> T -> rel var n2) (a : relOpen C n1) (b : T) : relOpen C n2 :=
+    match C with
       | nil => _
-      | nv :: R' => _ (@liftToOpen6 R' n1 T n2)
+      | nv :: C' => _ (@liftToOpen6 C' n1 T n2)
     end.
   Next Obligation.
     exact (f a b).
@@ -329,69 +367,69 @@ Section relOpen.
     exact (x f (a X) b).
   Defined.
 
-  Variable R : list nat.
+  Variable C : Ctx.
 
-  Definition ORvar n := liftToOpen3 R (@Rvar var n).
-  Definition ORlift := liftToOpen3 R (@Rlift var).
-  Definition ORtrue := liftToOpen4 R (@Rtrue var).
-  Definition ORfalse := liftToOpen4 R (@Rfalse var).
-  Definition ORand := liftToOpen5 R (@Rand var).
-  Definition ORor := liftToOpen5 R (@Ror var).
-  Definition ORimply := liftToOpen5 R (@Rimply var).
-  Definition ORforalle := liftToOpen2 R (@Rforalle var).
-  Definition ORexistse := liftToOpen2 R (@Rexistse var).
-  Definition ORforallR n := liftToOpen2 R (@RforallR var n).
-  Definition ORexistsR n := liftToOpen2 R (@RexistsR var n).
-  Definition ORforall1 T := liftToOpen2 R (@Rforall1 var T).
-  Definition ORexists1 T := liftToOpen2 R (@Rexists1 var T).
-  Definition ORabs n := liftToOpen2 R (@Rabs var n).
-  Definition ORapp n := liftToOpen6 R (@Rapp var n).
-  Definition ORrecur n := liftToOpen2 R (@Rrecur var n).
-  Definition ORlater := liftToOpen R (@Rlater var).
+  Definition ORvar n := liftToOpen3 C (@Rvar var n).
+  Definition ORinj := liftToOpen3 C (@Rinj var).
+  Definition ORtrue := liftToOpen4 C (@Rtrue var).
+  Definition ORfalse := liftToOpen4 C (@Rfalse var).
+  Definition ORand := liftToOpen5 C (@Rand var).
+  Definition ORor := liftToOpen5 C (@Ror var).
+  Definition ORimply := liftToOpen5 C (@Rimply var).
+  Definition ORforalle := liftToOpen2 C (@Rforalle var).
+  Definition ORexistse := liftToOpen2 C (@Rexistse var).
+  Definition ORforallR n := liftToOpen2 C (@RforallR var n).
+  Definition ORexistsR n := liftToOpen2 C (@RexistsR var n).
+  Definition ORforall1 T := liftToOpen2 C (@Rforall1 var T).
+  Definition ORexists1 T := liftToOpen2 C (@Rexists1 var T).
+  Definition ORabs n := liftToOpen2 C (@Rabs var n).
+  Definition ORapp n := liftToOpen6 C (@Rapp var n).
+  Definition ORrecur n := liftToOpen2 C (@Rrecur var n).
+  Definition ORlater := liftToOpen C (@Rlater var).
 
 End relOpen.
     
 Notation "⊤" := (ORtrue _ _).
 Notation "⊥" := (ORtrue _ _).
-Notation "⌈ P ⌉" := (ORlift _ _ P).
-Arguments ORabs {var R n} _ .
+Notation "⌈ P ⌉" := (ORinj _ _ P).
+Arguments ORabs {var C n} _ .
 Notation "\ x .. y , p" := (ORabs (fun x => .. (ORabs (fun y => p)) ..)) (at level 200, x binder, y binder, right associativity).
-Arguments ORforalle {var R} _ .
+Arguments ORforalle {var C} _ .
 Notation "∀ x .. y , p" := (ORforalle (fun x => .. (ORforalle (fun y => p)) ..)) (at level 200, x binder, y binder, right associativity).
-Arguments ORexistse {var R} _ .
+Arguments ORexistse {var C} _ .
 Notation "∃ x .. y , p" := (ORexistse (fun x => .. (ORexistse (fun y => p)) ..)) (at level 200, x binder, y binder, right associativity).
-Arguments ORforall1 {var R T} _ .
+Arguments ORforall1 {var C T} _ .
 Notation "∀1 x .. y , p" := (ORforall1 (fun x => .. (ORforall1 (fun y => p)) ..)) (at level 200, x binder, y binder, right associativity).
-Arguments ORexists1 {var R T} _ .
+Arguments ORexists1 {var C T} _ .
 Notation "∃1 x .. y , p" := (ORexists1 (fun x => .. (ORexists1 (fun y => p)) ..)) (at level 200, x binder, y binder, right associativity).
-Definition ORforallR' {var R n} P := (@ORforallR var R n (fun x => P (ORvar var R _ x))).
+Definition ORforallR' {var C n} P := (@ORforallR var C n (fun x => P (ORvar var C _ x))).
 Notation "∀2 x .. y , p" := (ORforallR' (fun x => .. (ORforallR' (fun y => p)) ..)) (at level 200, x binder, y binder, right associativity).
-Definition ORexistsR' {var R n} P := (@ORexistsR var R n (fun x => P (ORvar var R _ x))).
+Definition ORexistsR' {var C n} P := (@ORexistsR var C n (fun x => P (ORvar var C _ x))).
 Notation "∃2 x .. y , p" := (ORexistsR' (fun x => .. (ORexistsR' (fun y => p)) ..)) (at level 200, x binder, y binder, right associativity).
-Definition ORrecur' {var R n} P := (@ORrecur var R n (fun x => P (ORvar var R _ x))).
+Definition ORrecur' {var C n} P := (@ORrecur var C n (fun x => P (ORvar var C _ x))).
 Notation "@ x .. y , p" := (ORrecur' (fun x => .. (ORrecur' (fun y => p)) ..)) (at level 200, x binder, y binder, right associativity).
-Arguments ORapp {var R n} _ _ .
+Arguments ORapp {var C n} _ _ .
 Notation "e ∈ P" := (ORapp P e) (at level 70).
-Arguments ORand {var R} _ _ .
+Arguments ORand {var C} _ _ .
 Infix "/\" := ORand.
-Arguments ORor {var R} _ _ .
+Arguments ORor {var C} _ _ .
 Infix "\/" := ORor.
-Arguments ORimply {var R} _ _ .
+Arguments ORimply {var C} _ _ .
 Infix "⇒" := ORimply (at level 90).
-Arguments ORlater {var R} _ .
+Arguments ORlater {var C} _ .
 Notation "▹" := ORlater.
-Definition VSet {var R} τ (S : relOpen var R 1) := ∀ v, v ∈ S ⇒ ⌈v ↓ τ⌉.
+Definition VSet {var C} τ (S : relOpen var C 1) := ∀ v, v ∈ S ⇒ ⌈v ↓ τ⌉.
 
 Section TestNotations.
   
   Variable var : nat -> Type.
-  Variable R : list nat.
+  Variable C : Ctx.
 
-  Definition ttt1 : relOpen var R 1 := \e , ⊤.
-  Definition ttt2 : relOpen var R 1 := \e , ⌈e ↓ Tunit⌉.
-  Definition ttt3 : relOpen var R 1 := \_ , ⌈True /\ True⌉.
-  Definition ttt4 : relOpen var R 1 := \_ , ∀ e, ⌈e = Ett⌉.
-  Definition ttt5 : relOpen var R 1 := \_ , ∃ e, ⌈e = Ett⌉.
+  Definition ttt1 : relOpen var C 1 := \e , ⊤.
+  Definition ttt2 : relOpen var C 1 := \e , ⌈e ↓ Tunit⌉.
+  Definition ttt3 : relOpen var C 1 := \_ , ⌈True /\ True⌉.
+  Definition ttt4 : relOpen var C 1 := \_ , ∀ e, ⌈e = Ett⌉.
+  Definition ttt5 : relOpen var C 1 := \_ , ∃ e, ⌈e = Ett⌉.
 
 End TestNotations.
 
@@ -411,11 +449,14 @@ Local Open Scope prog_scope.
 Section LR.
   
   Variable var : nat -> Type.
-  Variable R : list nat.
+  Variable C : Ctx.
 
-  Definition substs : Type.
-    admit.
-  Defined.
+  Inductive SubstEntry :=
+  | SEtype (_ : relOpen var C (TTother type)) (_ : option (relOpen var C 1))
+  | SEexpr (_ : relOpen var C TTexpr) (_ : relOpen var C (TTother csize))
+  .
+
+  Definition substs : Type := list SubstEntry.
 
   Definition substs_type : substs -> type -> type.
     admit.
@@ -423,11 +464,11 @@ Section LR.
 
   Coercion substs_type : substs >-> Funclass.
 
-  Definition substs_sem : substs -> nat -> relOpen var R 1.
+  Definition substs_sem : substs -> nat -> relOpen var C 1.
     admit.
   Defined.
 
-  Instance Apply_substs_nat_rel : Apply substs nat (relOpen var R 1) :=
+  Instance Apply_substs_nat_rel : Apply substs nat (relOpen var C 1) :=
     {
       apply := substs_sem
     }.
@@ -459,28 +500,28 @@ Section LR.
       add := add_csize
     }.
 
-  Definition add_pair : (type * relOpen var R 1) -> substs -> substs.
+  Definition add_pair : (type * relOpen var C 1) -> substs -> substs.
     admit.
   Defined.
 
-  Instance Add_pair_substs : Add (type * relOpen var R 1) substs substs :=
+  Instance Add_pair_substs : Add (type * relOpen var C 1) substs substs :=
     {
       add := add_pair
     }.
 
-  Definition E' V τ (c : cexpr) (s : size) (ρ : substs) C (θ : thresholds) : relOpen var R 1 :=
-    \e, ∀ v, ∀1 n, ⌈|~ [] e (ρ τ) /\ ⇓ e n v⌉ ⇒ ⌈ ⌊ ñ | n ≤ C * ñ ⌋ (ρ $ c) ⌉ /\ ∃1 ξ : csize, ⌈ξ ≤ ρ $$ s⌉ /\ v ∈ V τ ξ ρ C θ.
+  Definition E' V τ (c : cexpr) (s : size) (ρ : substs) Ct (θ : thresholds) : relOpen var C 1 :=
+    \e, ∀ v, ∀1 n, ⌈|~ [] e (ρ τ) /\ ⇓ e n v⌉ ⇒ ⌈ ⌊ ñ | n ≤ Ct * ñ ⌋ (ρ $ c) ⌉ /\ ∃1 ξ : csize, ⌈ξ ≤ ρ $$ s⌉ /\ v ∈ V τ ξ ρ Ct θ.
 
-  Fixpoint V τ (ξ : csize) (ρ : substs) (C : nat) (θ : thresholds) {struct τ} : relOpen var R 1 :=
+  Fixpoint V τ (ξ : csize) (ρ : substs) (Ct : nat) (θ : thresholds) {struct τ} : relOpen var C 1 :=
     match τ, ξ, θ with
       | Tvar α, _, _ => ρ $ α
       | Tunit, _, _ => \v, ⌈v ↓ τ⌉
-      | τ₁ × τ₂, CSpair ξ₁ ξ₂, _ => \v, ⌈v ↓ ρ τ⌉ /\ ∃ a b, ⌈v = Epair a b⌉ /\ a ∈ V τ₁ ξ₁ ρ C θ /\ b ∈ V τ₂ ξ₂ ρ C θ
-      | τ₁ + τ₂, CSinl ξ, _ => \v, ⌈v ↓ ρ τ⌉ /\ ∃ v', ⌈v = Einl τ₂ v'⌉ /\ v' ∈ V τ₁ ξ ρ C θ
-      | τ₁ + τ₂, CSinr ξ, _ => \v, ⌈v ↓ ρ τ⌉ /\ ∃ v', ⌈v = Einr τ₁ v'⌉ /\ v' ∈ V τ₂ ξ ρ C θ
-      | Tarrow τ₁ c s τ₂, _, THarrow θ₁ ξ₀ θ₂ => \v, ⌈v ↓ ρ τ⌉ /\ ∀1 ξ₁, ∀ v₁, v₁ ∈ V τ₁ ξ₁ ρ C θ /\ ⌈ξ₀ ≤ |v₁|⌉ ⇒ Eapp v v₁ ∈ E' V τ₂ c s (add ξ₁ ρ) C θ₂
-      | Tuniversal c s τ, _, _ => \v, ⌈v ↓ ρ τ⌉ /\ ∀1 τ', ∀2 S, VSet τ' S ⇒ Etapp v τ' ∈ E' V τ c s (add (τ', S) ρ) C θ
-      | Trecur τ, CSfold ξ, _ => @S, \v, ⌈v ↓ ρ τ⌉ /\ ∃ v', ⌈v = Efold τ v'⌉ /\ ▹ (v' ∈ V τ ξ (add (ρ τ, S) ρ) C θ)
+      | τ₁ × τ₂, CSpair ξ₁ ξ₂, _ => \v, ⌈v ↓ ρ τ⌉ /\ ∃ a b, ⌈v = Epair a b⌉ /\ a ∈ V τ₁ ξ₁ ρ Ct θ /\ b ∈ V τ₂ ξ₂ ρ Ct θ
+      | τ₁ + τ₂, CSinl ξ, _ => \v, ⌈v ↓ ρ τ⌉ /\ ∃ v', ⌈v = Einl τ₂ v'⌉ /\ v' ∈ V τ₁ ξ ρ Ct θ
+      | τ₁ + τ₂, CSinr ξ, _ => \v, ⌈v ↓ ρ τ⌉ /\ ∃ v', ⌈v = Einr τ₁ v'⌉ /\ v' ∈ V τ₂ ξ ρ Ct θ
+      | Tarrow τ₁ c s τ₂, _, THarrow θ₁ ξ₀ θ₂ => \v, ⌈v ↓ ρ τ⌉ /\ ∀1 ξ₁, ∀ v₁, v₁ ∈ V τ₁ ξ₁ ρ Ct θ /\ ⌈ξ₀ ≤ |v₁|⌉ ⇒ Eapp v v₁ ∈ E' V τ₂ c s (add ξ₁ ρ) Ct θ₂
+      | Tuniversal c s τ, _, _ => \v, ⌈v ↓ ρ τ⌉ /\ ∀1 τ', ∀2 S, VSet τ' S ⇒ Etapp v τ' ∈ E' V τ c s (add (τ', S) ρ) Ct θ
+      | Trecur τ, CSfold ξ, _ => @S, \v, ⌈v ↓ ρ τ⌉ /\ ∃ v', ⌈v = Efold τ v'⌉ /\ ▹ (v' ∈ V τ ξ (add (ρ τ, S) ρ) Ct θ)
       | _, _, _ => \_, ⊥
     end
   .
@@ -488,47 +529,88 @@ Section LR.
   Definition E := E' V.
 
 End LR.
-*)
-Definition sound_wrt_bounded :=
-  forall f τ₁ c s τ₂, 
-    |~ [] f (Tarrow τ₁ c s τ₂) -> 
-    exists (C : nat) (ξ₀ : csize), 
-      (* ξ₀ is the threshold of input size in asymptotics *)
-      forall v,
-        v ↓ τ₁ ->
-        let ξ := |v| in
-        ξ₀ <= ξ ->
-        forall v' n, 
-          (* n is the actual running time *)
-          ⇓ (Eapp f v) n v' ->
-          (* n is bounded by c(ξ) w.r.t. constant factor C *)
-          ⌊ ñ | n <= C * ñ ⌋ (subst ξ c).
 
-Definition valid (X : list bool) {var} R (ctxP : list (relOpen var R 0)) (P : relOpen var R 0) : Prop.
+End OpenPHOAS.
+
+Import OpenPHOAS.
+
+Definition valid (X : list bool) {var} C (ctxP : list (relOpen var C 0)) (P : relOpen var C 0) : Prop.
   admit.
 Defined.
-Notation "|- X R ctxP P" := (valid X R ctxP P) (at level 90).
+Notation "|- X C ctxP P" := (valid X C ctxP P) (at level 90).
+
+Definition add_var t ctx Ps ρ :=
+  let ctx := t :: ctx in 
+  let Ps := lift t Ps in
+  let ρ := lift t ρ in
+  (ctx, Ps, ρ)
+.
+
+Definition add_type k :=
+  let Pack ctx0 Ps ρ := C in
+  let (ctx, Ps, ρ) := add_var TTtype ctx0 Ps ρ in
+  let Ps := extend ctx0 (fun τ => kinding [] τ k) :: Ps in
+  match k with
+    | KDstar => 
+      let C := add_rel_var C in
+      let C := add_premise (fun τ S => VSet τ S) C in
+      let C := add_ρ_type #1 (Some #0) C in
+      C
+    | _ =>
+      let C := add_ρ_type #1 None C in
+      C
+  end.
+
+Definition add_expr τ θ os :=
+  let ρ := get_ρ C in
+  let C := add_expr C in
+  let C := add_premise (#0 ∈ V τ ρ Ct θ) C in
+  let C := add_csize C in
+  let C := add_ρ_expr #1 #0 in
+  match os with
+    | inl ξ =>
+      let C := add_premise (#0 = ξ ≤ |#1| ? |#1| : ξ) C in
+      C
+    | inr s =>
+      let C := add_premise (asCsize (fun ξ => #0 = ξ) (ρ $$ s)) C in
+      C
+  end
+
+Fixpoint makeC Γ :=
+  match Γ with
+    | nil => (nil, nil)
+    | e : Γ =>
+      let C := makeC Γ in
+      match e with
+        | TEkinging k =>
+          add_type k C
+        | TEtyping (τ, θ, os) =>
+          add_expr τ θ os C
+      end
+  end.
 
 Definition related Γ e τ c s :=
-  exists C ξ₀'s θ,
-    length ξₒ's = length Γ /\
+  exists C ξs θs θ Γ',
+    extendΓ Γ ξs θs = Some Γ' /\
+    let (C, ρ) := makeC Γ' in
+    C |- ∃1 n ξ, nat_of_cexpr c = Some n /\ csize_of_size s = Some ξ /\ (ρ $ e) ∈ E τ (C * n) ξ ρ C θ
     (* ⊢ Γ e τ c s /\ *)
     let X := map () Γ in
-    let R := map () Γ in
+    let C := map () Γ in
     let ρ := map () Γ in
     let ctxP := map () Γ in
-    |- X R ctxP (e ∈ E c s ρ C θ)
+    |- X C ctxP (e ∈ E c s ρ C θ)
       
 (*
 Section inferRules.
 
   Variable var : nat -> Type.
 
-  Variable R : list nat.
+  Variable C : list nat.
 
   Reserved Notation "C |- P" (at level 90).
   
-  Inductive valid : list (relOpen var R 0) -> relOpen var R 0 -> Prop :=
+  Inductive valid : list (relOpen var C 0) -> relOpen var C 0 -> Prop :=
   | RuleMono C P : C |- P -> C |- ▹P
   | RuleLob C P : ▹P :: C |- P -> C |- P
   | RuleLaterAnd1 C P Q : C |- ▹ (P /\ Q) -> C |- ▹P /\ ▹Q
@@ -541,10 +623,10 @@ Section inferRules.
 End inferRules.
 *)
 
-Definition Rel n := forall var R, relOpen var R n.
+Definition Rel n := forall var C, relOpen var C n.
 
-Definition relV τ ξ ρ C θ : Rel 1 := fun var R => V var R τ ξ ρ C θ.
-Definition relE τ c s ρ C θ : Rel 1 := fun var R => E var R τ c s ρ C θ.
+Definition relV τ ξ ρ C θ : Rel 1 := fun var C => V var C τ ξ ρ C θ.
+Definition relE τ c s ρ C θ : Rel 1 := fun var C => E var C τ c s ρ C θ.
 
 Lemma foundamental :
   forall Γ e τ c s,
